ECDSA types to it's definition, some cleaning wrt p256prime

code/experimental/P256/Hacl.Impl.LowLevel.fst
@@ -17,7 +17,7 @@ open FStar.Math.Lemmas
 open FStar.Mul
 
 inline_for_extraction
-let prime_buffer: x: ilbuffer uint64 (size 4) {witnessed #uint64 #(size 4) x (Lib.Sequence.of_list p256_prime_list) /\ recallable x /\ felem_seq_as_nat (Lib.Sequence.of_list (p256_prime_list)) == prime} = 
+let prime256_buffer: x: ilbuffer uint64 (size 4) {witnessed #uint64 #(size 4) x (Lib.Sequence.of_list p256_prime_list) /\ recallable x /\ felem_seq_as_nat (Lib.Sequence.of_list (p256_prime_list)) == prime256} = 
 createL_global p256_prime_list
 
 open FStar.Mul
@@ -228,43 +228,43 @@ let cmovznz4 cin x y r =
 
 #reset-options "--z3refresh --z3rlimit 200"
 
-val reduction_prime_2prime_impl: x: felem -> result: felem -> 
+val reduction_prime256_2prime256_impl: x: felem -> result: felem -> 
   Stack unit
     (requires fun h -> live h x /\ live h result /\ eq_or_disjoint x result)
     (ensures fun h0 _ h1 -> modifies1 result h0 h1 /\ 
       (
   let r = as_seq h1 result in 
   let x = as_seq h0 x in 
-  felem_seq_as_nat r == felem_seq_as_nat x % prime
+  felem_seq_as_nat r == felem_seq_as_nat x % prime256
       )
     )
 
 #reset-options "--z3refresh --z3rlimit 300"
 
-val lemma_reduction1: a: nat {a < pow2 256} -> r: nat{if a >= prime then r = a - prime else r = a} -> 
-  Lemma (r = a % prime)
+val lemma_reduction1: a: nat {a < pow2 256} -> r: nat{if a >= prime256 then r = a - prime256 else r = a} -> 
+  Lemma (r = a % prime256)
 
 let lemma_reduction1 a r = 
-  assert_norm (pow2 256 - prime < prime);
-  assert(if a >= prime then a - prime < prime else True);
-  assert(if a >= prime then r < prime else True);
-  assert(if a >= prime then r = a % prime else True);
-  assert(if a < prime then r < prime else True);
-  assert(if a < prime then r = a % prime else True);
-  assert(r = a % prime)
+  assert_norm (pow2 256 - prime256 < prime256);
+  assert(if a >= prime256 then a - prime256 < prime256 else True);
+  assert(if a >= prime256 then r < prime256 else True);
+  assert(if a >= prime256 then r = a % prime256 else True);
+  assert(if a < prime256 then r < prime256 else True);
+  assert(if a < prime256 then r = a % prime256 else True);
+  assert(r = a % prime256)
 
 
 
-let reduction_prime_2prime_impl x result = 
+let reduction_prime256_2prime256_impl x result = 
   push_frame();
   let tempBuffer = create (size 4) (u64 0) in 
-    recall_contents prime_buffer (Lib.Sequence.of_list p256_prime_list);
+    recall_contents prime256_buffer (Lib.Sequence.of_list p256_prime_list);
         let h0 = ST.get() in 
-    let c = sub4_il x prime_buffer tempBuffer in 
+    let c = sub4_il x prime256_buffer tempBuffer in 
       let h1 = ST.get() in 
-      assert(felem_seq_as_nat (as_seq h1 tempBuffer) = felem_seq_as_nat (as_seq h0 x) - prime + uint_v c * pow2 256);
+      assert(felem_seq_as_nat (as_seq h1 tempBuffer) = felem_seq_as_nat (as_seq h0 x) - prime256 + uint_v c * pow2 256);
 
-      assert(let x = felem_seq_as_nat (as_seq h0 x) in if x < prime then uint_v c = 1 else uint_v c = 0);
+      assert(let x = felem_seq_as_nat (as_seq h0 x) in if x < prime256 then uint_v c = 1 else uint_v c = 0);
     cmovznz4 c tempBuffer x result;
       let h2 = ST.get() in 
     lemma_reduction1 (felem_seq_as_nat (as_seq h0 x)) (felem_seq_as_nat (as_seq h2 result));
@@ -272,51 +272,51 @@ let reduction_prime_2prime_impl x result =
 
 
 inline_for_extraction noextract
-val reduction_prime_2prime_with_carry_impl: cin: uint64 -> x: felem -> result: felem ->
+val reduction_prime256_2prime256_with_carry_impl: cin: uint64 -> x: felem -> result: felem ->
   Stack unit 
     (requires fun h -> live h x /\ live h result /\  eq_or_disjoint x result /\ 
-      (let x = as_seq h x in  felem_seq_as_nat x + uint_v cin * pow2 256) < 2 * prime)
+      (let x = as_seq h x in  felem_seq_as_nat x + uint_v cin * pow2 256) < 2 * prime256)
     (ensures fun h0 _ h1 -> modifies1 result h0 h1 /\ 
       (
   let r = as_seq h1 result in 
   let x = as_seq h0 x in 
-  felem_seq_as_nat r = (felem_seq_as_nat x + uint_v cin * pow2 256) % prime
+  felem_seq_as_nat r = (felem_seq_as_nat x + uint_v cin * pow2 256) % prime256
       )
     )  
 
-val lemma_r1: a: nat -> Lemma (if a < prime then a % prime == a else True)
+val lemma_r1: a: nat -> Lemma (if a < prime256 then a % prime256 == a else True)
 
 let lemma_r1 a = ()
 
 
-let reduction_prime_2prime_with_carry_impl cin x result = 
+let reduction_prime256_2prime256_with_carry_impl cin x result = 
   push_frame();
     let tempBuffer = create (size 4) (u64 0) in 
     let tempBufferForSubborrow = create (size 1) (u64 0) in 
-    recall_contents prime_buffer (Lib.Sequence.of_list p256_prime_list);
+    recall_contents prime256_buffer (Lib.Sequence.of_list p256_prime_list);
       let h0  = ST.get() in 
-    let c = sub4_il x prime_buffer tempBuffer in
+    let c = sub4_il x prime256_buffer tempBuffer in
       let h1 = ST.get() in 
-	assert(let x = felem_seq_as_nat (as_seq h0 x) in if x < prime then uint_v c = 1 else uint_v c = 0);
-	assert(felem_seq_as_nat (as_seq h1 tempBuffer)  = felem_seq_as_nat (as_seq h0 x) - prime + uint_v c * pow2 256);
+	assert(let x = felem_seq_as_nat (as_seq h0 x) in if x < prime256 then uint_v c = 1 else uint_v c = 0);
+	assert(felem_seq_as_nat (as_seq h1 tempBuffer)  = felem_seq_as_nat (as_seq h0 x) - prime256 + uint_v c * pow2 256);
     let carry = sub_borrow c cin (u64 0) tempBufferForSubborrow in 
       assert(if uint_v cin > 0 then uint_v carry == 0 else if uint_v c = 0 then uint_v carry = 0 else uint_v carry = 1);
       cmovznz4 carry tempBuffer x result;
       let h3 = ST.get() in 
-      modulo_addition_lemma (felem_seq_as_nat (as_seq h3 result)) prime 1;
-      assert((felem_seq_as_nat (as_seq h3 result) + prime) % prime = (felem_seq_as_nat (as_seq h3 result)) % prime);
+      modulo_addition_lemma (felem_seq_as_nat (as_seq h3 result)) prime256 1;
+      assert((felem_seq_as_nat (as_seq h3 result) + prime256) % prime256 = (felem_seq_as_nat (as_seq h3 result)) % prime256);
       lemma_r1 (felem_seq_as_nat (as_seq h3 result));
       
       assert(let resultN = felem_seq_as_nat (as_seq h3 result) in 
 	if uint_v cin = 1 then 
 	  if uint_v c = 0 then 
-	    resultN = felem_seq_as_nat (as_seq h0 x) - prime /\
-	    (felem_seq_as_nat (as_seq h0 x) + uint_v cin * pow2 256) % prime = resultN
+	    resultN = felem_seq_as_nat (as_seq h0 x) - prime256 /\
+	    (felem_seq_as_nat (as_seq h0 x) + uint_v cin * pow2 256) % prime256 = resultN
 	  else 
-	    resultN = felem_seq_as_nat (as_seq h0 x) - prime + pow2 256 /\
-	    resultN < prime /\
-	    resultN % prime == resultN  /\
-	    (felem_seq_as_nat (as_seq h0 x) + uint_v cin * pow2 256) % prime == resultN  
+	    resultN = felem_seq_as_nat (as_seq h0 x) - prime256 + pow2 256 /\
+	    resultN < prime256 /\
+	    resultN % prime256 == resultN  /\
+	    (felem_seq_as_nat (as_seq h0 x) + uint_v cin * pow2 256) % prime256 == resultN  
        else 
         True );
 
@@ -324,12 +324,12 @@ let reduction_prime_2prime_with_carry_impl cin x result =
 	if uint_v cin = 0 then 
 	  if uint_v c = 0 then 
 	    uint_v carry = 0 /\
-	    resultN = felem_seq_as_nat (as_seq h0 x) - prime /\
-	    (felem_seq_as_nat (as_seq h0 x) + uint_v carry * pow2 256) % prime  == resultN
+	    resultN = felem_seq_as_nat (as_seq h0 x) - prime256 /\
+	    (felem_seq_as_nat (as_seq h0 x) + uint_v carry * pow2 256) % prime256  == resultN
 	  else 
 	    uint_v carry = 1 /\
 	    resultN = felem_seq_as_nat (as_seq h0 x) /\
-	    (felem_seq_as_nat (as_seq h0 x) + uint_v cin * pow2 256) % prime  = resultN % prime 
+	    (felem_seq_as_nat (as_seq h0 x) + uint_v cin * pow2 256) % prime256  = resultN % prime256 
 	  else True  );
  
  pop_frame()   
@@ -372,7 +372,7 @@ val lemma_t_computation: t: uint64{uint_v t == 0 \/ uint_v t == 1} ->
   let t2 = (u64 0) -. t in 
   let t3 = (t <<. (size 32)) -. (t <<. (size 1)) in 
   let s = uint_v t0 + uint_v t1 * pow2 64 + uint_v t2 * pow2 128 + uint_v t3 * pow2 192 in 
-  if uint_v t = 1 then s == pow2 256 - prime - 1 else s == 0
+  if uint_v t = 1 then s == pow2 256 - prime256 - 1 else s == 0
     )
 
 let lemma_t_computation t = 
@@ -387,7 +387,7 @@ let lemma_t_computation t =
   assert_norm(if uint_v t = 1 then uint_v t2 = 18446744073709551615 else uint_v t2 = 0);
   assert_norm(if uint_v t = 1 then uint_v t3 = 4294967294 else uint_v t3 = 0);
  
-  assert_norm(18446744069414584320 * pow2 64 + 18446744073709551615 * pow2 128 + 4294967294 * pow2 192 = pow2 256 - prime - 1)
+  assert_norm(18446744069414584320 * pow2 64 + 18446744073709551615 * pow2 128 + 4294967294 * pow2 192 = pow2 256 - prime256 - 1)
 
 
 val lemma_t_computation2: t: uint64 {uint_v t == 0 \/ uint_v t == 1} ->
@@ -398,7 +398,7 @@ val lemma_t_computation2: t: uint64 {uint_v t == 0 \/ uint_v t == 1} ->
       let t2 = u64 0 in 
       let t3 = t -. (t <<. (size 32)) in 
       let s = uint_v t0 + uint_v t1 * pow2 64 + uint_v t2 * pow2 128 + uint_v t3 * pow2 192 in 
-  if uint_v t = 1 then s == prime else s == 0
+  if uint_v t = 1 then s == prime256 else s == 0
     )
 
 let lemma_t_computation2 t = 
@@ -413,7 +413,7 @@ let lemma_t_computation2 t =
   assert_norm(if uint_v t = 1 then uint_v t1 == 4294967295 else uint_v t1 = 0);
   assert_norm(if uint_v t = 1 then uint_v t3 == 18446744069414584321 else uint_v t3 = 0);
 
-  assert_norm(18446744073709551615 + 4294967295 * pow2 64 + 18446744069414584321 * pow2 192 = prime)
+  assert_norm(18446744073709551615 + 4294967295 * pow2 64 + 18446744069414584321 * pow2 192 = prime256)
 
 
 #set-options "--z3rlimit 500" 
@@ -422,7 +422,7 @@ val p256_add: arg1: felem -> arg2: felem ->  out: felem -> Stack unit
     live h0 arg1 /\ live h0 arg2 /\ live h0 out /\ eq_or_disjoint arg1 out /\ eq_or_disjoint arg2 out /\
     (
       let arg1_as_seq = as_seq h0 arg1 in let arg2_as_seq = as_seq h0 arg2 in 
-      felem_seq_as_nat arg1_as_seq < prime /\ felem_seq_as_nat arg2_as_seq < prime 
+      felem_seq_as_nat arg1_as_seq < prime256 /\ felem_seq_as_nat arg2_as_seq < prime256 
     )
    )
   )
@@ -431,7 +431,7 @@ val p256_add: arg1: felem -> arg2: felem ->  out: felem -> Stack unit
       let x = as_seq h0 arg1 in  
       let y = as_seq h0 arg2 in 
       let out = as_seq h1 out in 
-      felem_seq_as_nat out == (felem_seq_as_nat x + felem_seq_as_nat y) % prime /\
+      felem_seq_as_nat out == (felem_seq_as_nat x + felem_seq_as_nat y) % prime256 /\
       out == felem_add_seq (as_seq h0 arg1) (as_seq h0 arg2)
     )
   ))
@@ -444,9 +444,9 @@ let p256_add arg1 arg2 out =
       assert(let out = as_seq h1 out in let x = as_seq h0 arg1 in let y = as_seq h0 arg2 in 
       felem_seq_as_nat out + uint_v t * pow2 256 == felem_seq_as_nat x + felem_seq_as_nat y);
   lemma_t_computation t;
-  reduction_prime_2prime_with_carry_impl t out out;
+  reduction_prime256_2prime256_with_carry_impl t out out;
     let h2 = ST.get() in 
-    assert(felem_seq_as_nat (as_seq h2 out) == (felem_seq_as_nat (as_seq h0 arg1) + felem_seq_as_nat (as_seq h0 arg2)) % prime);
+    assert(felem_seq_as_nat (as_seq h2 out) == (felem_seq_as_nat (as_seq h0 arg1) + felem_seq_as_nat (as_seq h0 arg2)) % prime256);
     additionInDomain2Nat (felem_seq_as_nat (as_seq h0 arg1)) (felem_seq_as_nat (as_seq h0 arg2));
     inDomain_mod_is_not_mod (fromDomain_ (felem_seq_as_nat (as_seq h0 arg1)) + fromDomain_ (felem_seq_as_nat (as_seq h0 arg2)));
     lemma_eq_funct (as_seq h2 out) (felem_add_seq (as_seq h0 arg1) (as_seq h0 arg2))
@@ -456,15 +456,15 @@ let p256_add arg1 arg2 out =
 val p256_double: arg1: felem ->  out: felem -> Stack unit 
   (requires (fun h0 ->  live h0 arg1 /\ live h0 out /\  eq_or_disjoint arg1 out /\
     (
-      let arg1_as_seq = as_seq h0 arg1 in felem_seq_as_nat arg1_as_seq < prime
+      let arg1_as_seq = as_seq h0 arg1 in felem_seq_as_nat arg1_as_seq < prime256
     )
   ))
   (ensures (fun h0 _ h1 -> modifies1 out h0 h1 /\ 
     (
       let x = as_seq h0 arg1 in 
       let out = as_seq h1 out in 
-      felem_seq_as_nat out == (2 * felem_seq_as_nat x) % prime /\
-      felem_seq_as_nat out < prime
+      felem_seq_as_nat out == (2 * felem_seq_as_nat x) % prime256 /\
+      felem_seq_as_nat out < prime256
     )
   ))
 
@@ -477,7 +477,7 @@ let p256_double arg1 out =
       assert(let out = as_seq h1 out in let x = as_seq h0 arg1 in 
       felem_seq_as_nat out + uint_v t * pow2 256 == felem_seq_as_nat x + felem_seq_as_nat x);
   lemma_t_computation t;
-  reduction_prime_2prime_with_carry_impl t out out;
+  reduction_prime256_2prime256_with_carry_impl t out out;
   pop_frame()
 
 
@@ -485,13 +485,13 @@ let p256_double arg1 out =
 val p256_sub: arg1: felem -> arg2: felem -> out: felem -> Stack unit 
   (requires 
     (fun h0 -> live h0 out /\ live h0 arg1 /\ live h0 arg2 /\ eq_or_disjoint arg1 out /\ eq_or_disjoint arg2 out /\
-    as_nat h0 arg1 < prime /\ as_nat h0 arg2 < prime))
+    as_nat h0 arg1 < prime256 /\ as_nat h0 arg2 < prime256))
     (ensures (fun h0 _ h1 -> modifies1 out h0 h1 /\ 
       (
 	let x = as_seq h0 arg1 in 
 	let y = as_seq h0 arg2 in 
 	let out = as_seq h1 out in 
-	felem_seq_as_nat out == (felem_seq_as_nat x - felem_seq_as_nat y) % prime /\
+	felem_seq_as_nat out == (felem_seq_as_nat x - felem_seq_as_nat y) % prime256 /\
 	out == felem_sub_seq (as_seq h0 arg1) (as_seq h0 arg2)
       )
   ))
@@ -510,9 +510,9 @@ let p256_sub arg1 arg2 out =
   let t1 = ((u64 0) -. t) >>. (size 32) in 
   let t2 = u64 0 in 
   let t3 = t -. (t <<. (size 32)) in 
-    assert(if uint_v t = 1 then uint_v t0 + uint_v t1 * pow2 64 + uint_v t2 * pow2 128 + uint_v t3 * pow2 192 == prime else True);
-    modulo_addition_lemma  (let x = as_seq h0 arg1 in let y = as_seq h0 arg2 in (felem_seq_as_nat x - felem_seq_as_nat y)) prime 1;
-    assert(let x = as_seq h0 arg1 in let y = as_seq h0 arg2 in  (felem_seq_as_nat x - felem_seq_as_nat y + prime) % prime = (felem_seq_as_nat x - felem_seq_as_nat y) % prime);
+    assert(if uint_v t = 1 then uint_v t0 + uint_v t1 * pow2 64 + uint_v t2 * pow2 128 + uint_v t3 * pow2 192 == prime256 else True);
+    modulo_addition_lemma  (let x = as_seq h0 arg1 in let y = as_seq h0 arg2 in (felem_seq_as_nat x - felem_seq_as_nat y)) prime256 1;
+    assert(let x = as_seq h0 arg1 in let y = as_seq h0 arg2 in  (felem_seq_as_nat x - felem_seq_as_nat y + prime256) % prime256 = (felem_seq_as_nat x - felem_seq_as_nat y) % prime256);
 
   let c = add4_variables out (u64 0)  t0 t1 t2 t3 out in 
     let h2 = ST.get() in 
@@ -521,13 +521,13 @@ let p256_sub arg1 arg2 out =
       let s = uint_v t0 + uint_v t1 * pow2 64 + uint_v t2 * pow2 128 + uint_v t3 * pow2 192 in 
       if felem_seq_as_nat x - felem_seq_as_nat y >= 0 then 
       begin
-	  modulo_lemma (felem_seq_as_nat x - felem_seq_as_nat y) prime;
-	  felem_seq_as_nat result == (felem_seq_as_nat x - felem_seq_as_nat y) % prime
+	  modulo_lemma (felem_seq_as_nat x - felem_seq_as_nat y) prime256;
+	  felem_seq_as_nat result == (felem_seq_as_nat x - felem_seq_as_nat y) % prime256
       end
       else
           begin
-	    modulo_lemma (felem_seq_as_nat result) prime;
-            felem_seq_as_nat result == (felem_seq_as_nat x - felem_seq_as_nat y) % prime
+	    modulo_lemma (felem_seq_as_nat result) prime256;
+            felem_seq_as_nat result == (felem_seq_as_nat x - felem_seq_as_nat y) % prime256
 	  end
   );
 
