code/experimental/P256/Hacl.Impl.MontgomeryMultiplication.fst
@@ -10,15 +10,13 @@ open Lib.Buffer
 open FStar.Math.Lemmas
 
 open Hacl.Spec.P256.Lemmas
-open Hacl.Spec.P256.Definitions
+open Hacl.Spec.ECDSAP256.Definition
 open Hacl.Impl.LowLevel
 open Hacl.Spec.P256.Basic
 open Hacl.Spec.P256.Core
 
 open FStar.Mul
 
-noextract
-let prime:pos = 115792089210356248762697446949407573529996955224135760342422259061068512044369
 
 #reset-options "--z3refresh --z3rlimit 200"
 inline_for_extraction noextract
@@ -129,20 +127,20 @@ let shortened_mul a b result =
 
 inline_for_extraction noextract
 val add8_without_carry:
-  a: felem8 {wide_as_nat4 a < prime * prime} -> 
+  a: felem8 {wide_as_nat4 a < prime_p256_order * prime_p256_order} -> 
   b: felem8 {wide_as_nat4 b < pow2 320}  -> Tot (r:felem8 {wide_as_nat4 r = wide_as_nat4 a + wide_as_nat4 b})
 
 
 let add8_without_carry (a0, a1, a2, a3, a4, a5, a6, a7) (b0, b1, b2, b3, b4, b5, b6, b7) = 
   let (carry, r0, r1, r2, r3, r4, r5, r6, r7)  = add8 (a0, a1, a2, a3, a4, a5, a6, a7) (b0, b1, b2, b3, b4, b5, b6, b7) in 
-  assert_norm (pow2 320 +  prime * prime  < pow2 512);
+  assert_norm (pow2 320 +  prime_p256_order * prime_p256_order  < pow2 512);
   assert(uint_v carry = 0);
   (r0, r1, r2, r3, r4, r5, r6, r7)
 
 
 val add8_without_carry1:  t: widefelem -> t1: widefelem -> result: widefelem  -> Stack unit
   (requires fun h -> live h t /\ live h t1 /\ live h result /\ wide_as_nat h t1 < pow2 320 /\
-    wide_as_nat h t <  prime * prime  )
+    wide_as_nat h t <  prime_p256_order * prime_p256_order  )
   (ensures fun h0 _ h1 -> modifies1 result h0 h1 /\  wide_as_nat h1 result = wide_as_nat h0 t + wide_as_nat h0 t1)
 
 let add8_without_carry1 t r result  = 
@@ -201,35 +199,35 @@ private let add_l2 (a: int) (b: nat) (c: int) (d: nat) : Lemma (requires a <= c 
 private let div_lemma (a: int) (b: pos) (c: nat) : Lemma (requires a < b) (ensures a / b <= c / b) = ()
 
 
-val lemma_montgomery_mult_1: prime : pos {prime = 115792089210356248762697446949407573529996955224135760342422259061068512044369} -> 
-t : int  -> k0:nat {k0 = modp_inv2_prime (-prime) (pow2 64)} -> r: nat {t <= r} -> 
-Lemma (ensures (t + (((t % pow2 64) * k0) % pow2 64 * prime)) / pow2 64 <= (pow2 64 * prime + r) / pow2 64)
+val lemma_montgomery_mult_1: prime_p256_order : pos {prime_p256_order = 115792089210356248762697446949407573529996955224135760342422259061068512044369} -> 
+t : int  -> k0:nat {k0 = modp_inv2_prime (-prime_p256_order) (pow2 64)} -> r: nat {t <= r} -> 
+Lemma (ensures (t + (((t % pow2 64) * k0) % pow2 64 * prime_p256_order)) / pow2 64 <= (pow2 64 * prime_p256_order + r) / pow2 64)
 
 
-let lemma_montgomery_mult_1 prime t k0 r = 
+let lemma_montgomery_mult_1 prime_p256_order t k0 r = 
   let t1 = t % pow2 64 in 
     assert(t1 < pow2 64);
   let y = (t1 * k0) % pow2 64 in 
     assert(y < pow2 64);
-  let t2 = y * prime in 
-    mul_lemma_1 y (pow2 64) prime;
-    assert(t2 < pow2 64 * prime); 
+  let t2 = y * prime_p256_order in 
+    mul_lemma_1 y (pow2 64) prime_p256_order;
+    assert(t2 < pow2 64 * prime_p256_order); 
   let t3 = t + t2 in
-    add_l2 t t2 r (pow2 64 * prime); 
-    assert(t3 < (r + pow2 64 * prime));
+    add_l2 t t2 r (pow2 64 * prime_p256_order); 
+    assert(t3 < (r + pow2 64 * prime_p256_order));
   let t = t3 / pow2 64 in 
-    assert_norm (pow2 64 * prime + r > 0); 
-    div_lemma t3 (r + pow2 64 * prime) (pow2 64);
-    assert(t <= (pow2 64 * prime + r) / pow2 64); 
-    let r = (pow2 64 * prime + r) / pow2 64 in 
+    assert_norm (pow2 64 * prime_p256_order + r > 0); 
+    div_lemma t3 (r + pow2 64 * prime_p256_order) (pow2 64);
+    assert(t <= (pow2 64 * prime_p256_order + r) / pow2 64); 
+    let r = (pow2 64 * prime_p256_order + r) / pow2 64 in 
     assert(t <= r)
 
 
 
 
 #reset-options "--z3refresh --z3rlimit 300"
-val lemma_montgomery_mult_result_less_than_prime: 
-  a: nat{a < prime} -> b: nat{b < prime} -> k0:nat {k0 = modp_inv2_prime (-prime) (pow2 64)} -> 
+val lemma_montgomery_mult_result_less_than_prime_p256_order: 
+  a: nat{a < prime_p256_order} -> b: nat{b < prime_p256_order} -> k0:nat {k0 = modp_inv2_prime (-prime_p256_order) (pow2 64)} -> 
   Lemma
   (ensures (  
     let t = a * b in 
@@ -237,96 +235,96 @@ val lemma_montgomery_mult_result_less_than_prime:
   
     let t1 = t % pow2 s in 
     let y = (t1 * k0) % pow2 s in 
-    let t2 = y * prime in 
+    let t2 = y * prime_p256_order in 
     let t3 = t + t2 in
     let t = t3 / pow2 s in 
   
     let t1 = t % pow2 s in 
     let y = (t1 * k0) % pow2 s in 
-    let t2 = y * prime in 
+    let t2 = y * prime_p256_order in 
     let t3 = t + t2 in
     let t = t3 / pow2 s in 
   
     let t1 = t % pow2 s in 
     let y = (t1 * k0) % pow2 s in 
-    let t2 = y * prime in 
+    let t2 = y * prime_p256_order in 
     let t3 = t + t2 in
     let t = t3 / pow2 s in 
     
     let t1 = t % pow2 s in 
     let y = (t1 * k0) % pow2 s in 
-    let t2 = y * prime in 
+    let t2 = y * prime_p256_order in 
     let t3 = t + t2 in
     let t = t3 / pow2 s in 
-    t < 2 * prime))
+    t < 2 * prime_p256_order))
 
 
 
 
-let lemma_montgomery_mult_result_less_than_prime a b k0 = 
+let lemma_montgomery_mult_result_less_than_prime_p256_order a b k0 = 
   let t = a * b in 
   let s = 64 in 
-    mul_lemma_ a b prime;
+    mul_lemma_ a b prime_p256_order;
 
-  let r = prime * prime + 1 in 
+  let r = prime_p256_order * prime_p256_order + 1 in 
       assert(t <= r); 
-      assert(t < prime * prime);
+      assert(t < prime_p256_order * prime_p256_order);
 
   let t1 = t % pow2 s in 
   let y = (t1 * k0) % pow2 s in 
-  let t2 = y * prime in 
+  let t2 = y * prime_p256_order in 
   let t3 = t + t2 in
   let tU = t3 / pow2 s in 
-  lemma_montgomery_mult_1 prime t k0 r; 
+  lemma_montgomery_mult_1 prime_p256_order t k0 r; 
 
   let t = tU in 
-  let r = (pow2 64 * prime + r) / pow2 64 in 
+  let r = (pow2 64 * prime_p256_order + r) / pow2 64 in 
     let t1 = t % pow2 s in 
   let y = (t1 * k0) % pow2 s in 
-  let t2 = y * prime in 
+  let t2 = y * prime_p256_order in 
   let t3 = t + t2 in
   let tU = t3 / pow2 s in 
   
   assert(t <= r); 
-  lemma_montgomery_mult_1 prime t k0 r; 
+  lemma_montgomery_mult_1 prime_p256_order t k0 r; 
 
    let t = tU in 
-   let r = (pow2 64 * prime + r) / pow2 64 in 
+   let r = (pow2 64 * prime_p256_order + r) / pow2 64 in 
     
     let t1 = t % pow2 s in 
   let y = (t1 * k0) % pow2 s in 
-  let t2 = y * prime in 
+  let t2 = y * prime_p256_order in 
   let t3 = t + t2 in
   let tU = t3 / pow2 s in 
-  lemma_montgomery_mult_1 prime t k0 r; 
+  lemma_montgomery_mult_1 prime_p256_order t k0 r; 
 
-  let r = (pow2 64 * prime + r) / pow2 64 in 
+  let r = (pow2 64 * prime_p256_order + r) / pow2 64 in 
   let t = tU in 
 
     let t1 = t % pow2 s in 
   let y = (t1 * k0) % pow2 s in 
-  let t2 = y * prime in 
+  let t2 = y * prime_p256_order in 
   let t3 = t + t2 in
   let tU = t3 / pow2 s in 
-  lemma_montgomery_mult_1 prime t k0 r; 
+  lemma_montgomery_mult_1 prime_p256_order t k0 r; 
   
-  let r = (pow2 64 * prime + r) / pow2 64 in 
+  let r = (pow2 64 * prime_p256_order + r) / pow2 64 in 
   assert(tU <= r);
-  assert(tU <=  (pow2 64 * prime +  (pow2 64 * prime +  (pow2 64 * prime +  (pow2 64 * prime +  prime * prime + 1) / pow2 64) / pow2 64) / pow2 64) / pow2 64);
-  assert_norm ((pow2 64 * prime +  (pow2 64 * prime +  (pow2 64 * prime +  (pow2 64 * prime +  prime * prime + 1) / pow2 64) / pow2 64) / pow2 64) / pow2 64 < 2 * prime);
-  assert(tU < 2 * prime)
+  assert(tU <=  (pow2 64 * prime_p256_order +  (pow2 64 * prime_p256_order +  (pow2 64 * prime_p256_order +  (pow2 64 * prime_p256_order +  prime_p256_order * prime_p256_order + 1) / pow2 64) / pow2 64) / pow2 64) / pow2 64);
+  assert_norm ((pow2 64 * prime_p256_order +  (pow2 64 * prime_p256_order +  (pow2 64 * prime_p256_order +  (pow2 64 * prime_p256_order +  prime_p256_order * prime_p256_order + 1) / pow2 64) / pow2 64) / pow2 64) / pow2 64 < 2 * prime_p256_order);
+  assert(tU < 2 * prime_p256_order)
 
 
 val lemma_montgomery_mod_inverse_addition: a: nat -> 
   Lemma (
-    (a * modp_inv2_prime (pow2 64) prime  * modp_inv2_prime (pow2 64) prime) % prime == (a * modp_inv2_prime (pow2 128) prime) % prime)
+    (a * modp_inv2_prime(pow2 64) prime_p256_order  * modp_inv2_prime (pow2 64) prime_p256_order) % prime_p256_order == (a * modp_inv2_prime(pow2 128) prime_p256_order) % prime_p256_order)
 
 
 let lemma_montgomery_mod_inverse_addition a = admit()
 
 val lemma_montgomery_mod_inverse_addition2: a: nat -> 
   Lemma (
-    (a * modp_inv2_prime (pow2 128) prime  * modp_inv2_prime (pow2 128) prime) % prime == (a * modp_inv2_prime (pow2 256) prime) % prime)
+    (a * modp_inv2_prime (pow2 128) prime_p256_order  * modp_inv2_prime (pow2 128) prime_p256_order) % prime_p256_order == (a * modp_inv2_prime (pow2 256) prime_p256_order) % prime_p256_order)
 
 
 let lemma_montgomery_mod_inverse_addition2 a = admit()
@@ -337,23 +335,23 @@ let lemma_montgomery_mod_inverse_addition2 a = admit()
 
 val montgomery_multiplication_one_round_proof: 
   t: nat ->
-  k0: nat {k0 = modp_inv2_prime (-prime) (pow2 64)}  ->  
-  round: nat {round = (t + prime * ((k0 * (t % pow2 64)) % pow2 64)) / pow2 64} -> co: nat {co % prime = t % prime} -> 
-  Lemma (round  % prime == co * (modp_inv2_prime (pow2 64) prime) % prime )
+  k0: nat {k0 = modp_inv2_prime (-prime_p256_order) (pow2 64)}  ->  
+  round: nat {round = (t + prime_p256_order * ((k0 * (t % pow2 64)) % pow2 64)) / pow2 64} -> co: nat {co % prime_p256_order = t % prime_p256_order} -> 
+  Lemma (round  % prime_p256_order == co * (modp_inv2_prime (pow2 64) prime_p256_order) % prime_p256_order )
 
 let montgomery_multiplication_one_round_proof t k0 round co = 
-  mult_one_round_ecdsa_prime t prime co k0 
+  mult_one_round_ecdsa_prime t prime_p256_order co k0 
 
-val montgomery_multiplication_round: t: widefelem ->  round: widefelem -> k0: uint64 -> primeBuffer: lbuffer uint64 (size 4)  ->
+val montgomery_multiplication_round: t: widefelem ->  round: widefelem -> k0: uint64 -> prime_p256_orderBuffer: lbuffer uint64 (size 4)  ->
   Stack unit 
-    (requires fun h -> live h t /\ live h round /\ live h primeBuffer /\ as_nat h primeBuffer == prime /\
-      wide_as_nat h t < prime * prime)
+    (requires fun h -> live h t /\ live h round /\ live h prime_p256_orderBuffer /\ as_nat h prime_p256_orderBuffer == prime_p256_order /\
+      wide_as_nat h t < prime_p256_order * prime_p256_order)
     (ensures fun h0 _ h1 -> modifies1 round h0 h1 /\ 
-      wide_as_nat h1 round = (wide_as_nat h0 t + prime * ((uint_v k0 * (wide_as_nat h0 t % pow2 64)) % pow2 64) ) / pow2 64
+      wide_as_nat h1 round = (wide_as_nat h0 t + prime_p256_order * ((uint_v k0 * (wide_as_nat h0 t % pow2 64)) % pow2 64) ) / pow2 64
     )
 
 
-let montgomery_multiplication_round t round k0 primeBuffer = 
+let montgomery_multiplication_round t round k0 prime_p256_orderBuffer = 
   let open FStar.Tactics in 
   let open FStar.Tactics.Canon in 
   push_frame(); 
@@ -364,107 +362,107 @@ let montgomery_multiplication_round t round k0 primeBuffer =
     let t1 = mod64 t in 
     let y, _ = mul64 t1 k0 in 
       assert(uint_v y = uint_v t1 * uint_v k0 % pow2 64);
-    shortened_mul primeBuffer y t2;
+    shortened_mul prime_p256_orderBuffer y t2;
       let h2 = ST.get() in 
-      assert(wide_as_nat h2 t2 = prime * ((uint_v t1 * uint_v k0) % pow2 64)); 
+      assert(wide_as_nat h2 t2 = prime_p256_order * ((uint_v t1 * uint_v k0) % pow2 64)); 
     add8_without_carry1 t t2 t3;
       let h3 = ST.get() in 
       assert_by_tactic ((wide_as_nat h0 t % pow2 64) * uint_v k0 == uint_v k0 * (wide_as_nat h0 t % pow2 64)) canon;
-      assert(wide_as_nat h3 t3 == wide_as_nat h0 t + prime * ((uint_v k0 * (wide_as_nat h0 t % pow2 64))  % pow2 64));
+      assert(wide_as_nat h3 t3 == wide_as_nat h0 t + prime_p256_order * ((uint_v k0 * (wide_as_nat h0 t % pow2 64))  % pow2 64));
     shift8 t3 round;
       let h4 = ST.get() in 
   pop_frame()
 
 inline_for_extraction noextract
-val montgomery_multiplication_round_twice: t: widefelem -> result: widefelem -> k0: uint64 -> primeBuffer : felem -> 
+val montgomery_multiplication_round_twice: t: widefelem -> result: widefelem -> k0: uint64 -> prime_p256_orderBuffer : felem -> 
   Stack unit 
-    (requires fun h -> live h t /\ live h result /\ live h primeBuffer /\
-      wide_as_nat h t < prime * prime /\ as_nat h primeBuffer == prime /\
-	uint_v k0 == modp_inv2_prime (-prime) (pow2 64)
+    (requires fun h -> live h t /\ live h result /\ live h prime_p256_orderBuffer /\
+      wide_as_nat h t < prime_p256_order * prime_p256_order /\ as_nat h prime_p256_orderBuffer == prime_p256_order /\
+	uint_v k0 == modp_inv2_prime (-prime_p256_order) (pow2 64)
       )
     (ensures fun h0 _ h1 -> modifies1 result h0 h1 /\ 
-      wide_as_nat h1 result % prime == (wide_as_nat h0 t * modp_inv2_prime (pow2 128) prime) % prime /\
-      (let round = (wide_as_nat h0 t + prime * ((uint_v k0 * (wide_as_nat h0 t % pow2 64)) % pow2 64)) / pow2 64 in 
-	wide_as_nat h1 result == (round + prime * ((uint_v k0 * (round % pow2 64)) % pow2 64)) / pow2 64)  /\
-	wide_as_nat h1 result < prime * prime
+      wide_as_nat h1 result % prime_p256_order == (wide_as_nat h0 t * modp_inv2_prime (pow2 128) prime_p256_order) % prime_p256_order /\
+      (let round = (wide_as_nat h0 t + prime_p256_order * ((uint_v k0 * (wide_as_nat h0 t % pow2 64)) % pow2 64)) / pow2 64 in 
+	wide_as_nat h1 result == (round + prime_p256_order * ((uint_v k0 * (round % pow2 64)) % pow2 64)) / pow2 64)  /\
+	wide_as_nat h1 result < prime_p256_order * prime_p256_order
       )
     
 
-let montgomery_multiplication_round_twice t result k0 primeBuffer = 
+let montgomery_multiplication_round_twice t result k0 prime_p256_orderBuffer = 
    push_frame();
      let tempRound = create (size 8) (u64 0) in 
        let h0 = ST.get() in 
-     montgomery_multiplication_round t tempRound k0 primeBuffer; 
+     montgomery_multiplication_round t tempRound k0 prime_p256_orderBuffer; 
        let h1 = ST.get() in 
-       assert(wide_as_nat h1 tempRound == (wide_as_nat h0 t + prime * ((uint_v k0 * (wide_as_nat h0 t % pow2 64)) % pow2 64)) / pow2 64);
+       assert(wide_as_nat h1 tempRound == (wide_as_nat h0 t + prime_p256_order * ((uint_v k0 * (wide_as_nat h0 t % pow2 64)) % pow2 64)) / pow2 64);
        montgomery_multiplication_one_round_proof (wide_as_nat h0 t) (uint_v k0) (wide_as_nat h1 tempRound) (wide_as_nat h0 t);
-       assert(wide_as_nat h1 tempRound % prime == (wide_as_nat h0 t * modp_inv2_prime (pow2 64) prime) % prime);
+       assert(wide_as_nat h1 tempRound % prime_p256_order == (wide_as_nat h0 t * modp_inv2_prime (pow2 64) prime_p256_order) % prime_p256_order);
 
-    montgomery_multiplication_round tempRound result k0 primeBuffer; 
+    montgomery_multiplication_round tempRound result k0 prime_p256_orderBuffer; 
       let h2 = ST.get() in 
-      assert(let round = (wide_as_nat h0 t + prime * ((uint_v k0 * (wide_as_nat h0 t % pow2 64)) % pow2 64)) / pow2 64 in 
-	wide_as_nat h2 result == (round + prime * ((uint_v k0 * (round % pow2 64)) % pow2 64)) / pow2 64);
-      montgomery_multiplication_one_round_proof (wide_as_nat h1 tempRound) (uint_v k0) (wide_as_nat h2 result) (wide_as_nat h0 t * modp_inv2_prime (pow2 64) prime); 
-      assert(wide_as_nat h2 result % prime == (wide_as_nat h0 t * modp_inv2_prime (pow2 64) prime * modp_inv2_prime (pow2 64) prime) % prime);
+      assert(let round = (wide_as_nat h0 t + prime_p256_order * ((uint_v k0 * (wide_as_nat h0 t % pow2 64)) % pow2 64)) / pow2 64 in 
+	wide_as_nat h2 result == (round + prime_p256_order * ((uint_v k0 * (round % pow2 64)) % pow2 64)) / pow2 64);
+      montgomery_multiplication_one_round_proof (wide_as_nat h1 tempRound) (uint_v k0) (wide_as_nat h2 result) (wide_as_nat h0 t * modp_inv2_prime (pow2 64) prime_p256_order); 
+      assert(wide_as_nat h2 result % prime_p256_order == (wide_as_nat h0 t * modp_inv2_prime (pow2 64) prime_p256_order * modp_inv2_prime (pow2 64) prime_p256_order) % prime_p256_order);
       lemma_montgomery_mod_inverse_addition (wide_as_nat h0 t); 
-      assert((wide_as_nat h0 t * modp_inv2_prime (pow2 64) prime * modp_inv2_prime (pow2 64) prime) % prime ==
-	(wide_as_nat h0 t * modp_inv2_prime(pow2 128) prime) % prime);
+      assert((wide_as_nat h0 t * modp_inv2_prime (pow2 64) prime_p256_order * modp_inv2_prime (pow2 64) prime_p256_order) % prime_p256_order ==
+	(wide_as_nat h0 t * modp_inv2_prime(pow2 128) prime_p256_order) % prime_p256_order);
   pop_frame()
 
 
 
 inline_for_extraction noextract
-val reduction_prime_2prime_with_carry_impl_5: x: widefelem -> result: felem -> primeBuffer: felem -> 
+val reduction_prime_p256_order_2prime_p256_order_with_carry_impl_5: x: widefelem -> result: felem -> prime_p256_orderBuffer: felem -> 
   Stack unit 
-    (requires fun h -> live h x /\ live h result /\  eq_or_disjoint x result /\ live h primeBuffer /\
-      (as_nat h primeBuffer == prime) /\ wide_as_nat h x < 2 * prime)
-    (ensures fun h0 _ h1 -> modifies1 result h0 h1 /\ as_nat h1 result = wide_as_nat h0 x % prime)  
+    (requires fun h -> live h x /\ live h result /\  eq_or_disjoint x result /\ live h prime_p256_orderBuffer /\
+      (as_nat h prime_p256_orderBuffer == prime_p256_order) /\ wide_as_nat h x < 2 * prime_p256_order)
+    (ensures fun h0 _ h1 -> modifies1 result h0 h1 /\ as_nat h1 result = wide_as_nat h0 x % prime_p256_order)  
 
 
-let reduction_prime_2prime_with_carry_impl_5 x result primeBuffer  = 
+let reduction_prime_p256_order_2prime_p256_order_with_carry_impl_5 x result prime_p256_orderBuffer  = 
   push_frame();
     let tempBuffer = create (size 4) (u64 0) in 
     let tempBufferForSubborrow = create (size 1) (u64 0) in 
     let cin = Lib.Buffer.index x (size 4) in 
     let x = Lib.Buffer.sub x (size 0) (size 4) in 
-    let c = Hacl.Impl.LowLevel.sub4 x primeBuffer tempBuffer in
+    let c = Hacl.Impl.LowLevel.sub4 x prime_p256_orderBuffer tempBuffer in
     let carry = sub_borrow c cin (u64 0) tempBufferForSubborrow in 
     assert(if uint_v cin > 0 then uint_v carry == 0 else if uint_v c = 0 then uint_v carry = 0 else uint_v carry = 1);
     cmovznz4 carry tempBuffer x result;
  pop_frame()   
 
-val lemma_montgomery_mult_2: a: nat{a < prime} -> b: nat {b < prime} -> 
+val lemma_montgomery_mult_2: a: nat{a < prime_p256_order} -> b: nat {b < prime_p256_order} -> 
   Lemma (
-    (a * b *  modp_inv2_prime (pow2 64) prime  * 
-      modp_inv2_prime (pow2 64) prime  *
-      modp_inv2_prime (pow2 64) prime *
-      modp_inv2_prime (pow2 64) prime) % prime == (a * b *  modp_inv2_prime (pow2 256) prime) % prime)
+    (a * b *  modp_inv2_prime (pow2 64) prime_p256_order  * 
+      modp_inv2_prime (pow2 64) prime_p256_order  *
+      modp_inv2_prime (pow2 64) prime_p256_order *
+      modp_inv2_prime (pow2 64) prime_p256_order) % prime_p256_order == (a * b *  modp_inv2_prime (pow2 256) prime_p256_order) % prime_p256_order)
 
 
 let lemma_montgomery_mult_2 t = 
-    assert_norm (prime > 3);
-    assert_norm(modp_inv2_prime (pow2 64) prime  == 92642477083479937529731757477833778746952469466660261742446881162473064518108); admit()
+    assert_norm (prime_p256_order > 3);
+    assert_norm(modp_inv2_prime (pow2 64) prime_p256_order  == 92642477083479937529731757477833778746952469466660261742446881162473064518108); admit()
 
 
 
 
-val upload_ecdsa_prime: p: lbuffer uint64 (size 4) -> Stack unit
+val upload_ecdsa_prime_p256_order: p: lbuffer uint64 (size 4) -> Stack unit
   (requires fun h -> live h p)
-  (ensures fun h0 _ h1 -> modifies1 p h0 h1 /\ as_nat h1 p == prime)
+  (ensures fun h0 _ h1 -> modifies1 p h0 h1 /\ as_nat h1 p == prime_p256_order)
 
-let upload_ecdsa_prime p = 
+let upload_ecdsa_prime_p256_order p = 
   upd p (size 0) (u64 17562291160714782033);
   upd p (size 1) (u64 13611842547513532036);
   upd p (size 2) (u64 18446744073709551615);
   upd p (size 3) (u64 18446744069414584320)
 
-val upload_k0: unit ->  Tot (r: uint64 {uint_v r == modp_inv2_prime (-prime) (pow2 64)})
+val upload_k0: unit ->  Tot (r: uint64 {uint_v r == modp_inv2_prime (-prime_p256_order) (pow2 64)})
 
 let upload_k0 () = 
   (* 
   SAGE: 
   
-  prime = 115792089210356248762697446949407573529996955224135760342422259061068512044369
+  prime_p256_order = 115792089210356248762697446949407573529996955224135760342422259061068512044369
   inverse_mod(884452912994769583, 2**64)
 
      14758798090332847183  
@@ -474,11 +472,23 @@ let upload_k0 () =
 
 
 
+
+noextract
+val fromDomain_: a: nat -> Tot nat 
+
+let fromDomain_ a = (a * modp_inv2_prime (pow2 256) prime_p256_order) % prime_p256_order
+
+noextract
+val toDomain_: a: nat -> Tot nat
+let toDomain_ a = (a * pow2 256) % prime_p256_order 
+
+
 val montgomery_multiplication_ecdsa_module: a: felem -> b: felem ->result: felem-> 
   Stack unit 
     (requires fun h -> live h a /\ live h b /\ live h result /\
-      as_nat h a < prime /\ as_nat h b < prime)
-    (ensures fun h0 _ h1 -> modifies1 result h0 h1 /\ as_nat h1 result = (as_nat h0 a * as_nat h0 b * modp_inv2_prime (pow2 256) prime) % prime )
+      as_nat h a < prime_p256_order /\ as_nat h b < prime_p256_order)
+    (ensures fun h0 _ h1 -> modifies1 result h0 h1 /\ as_nat h1 result = (as_nat h0 a * as_nat h0 b * modp_inv2_prime (pow2 256) prime_p256_order) % prime_p256_order /\ 
+      as_nat h1 result = fromDomain_(as_nat h0 a * as_nat h0 b) )
 
 
 let montgomery_multiplication_ecdsa_module a b result =
@@ -486,29 +496,29 @@ let montgomery_multiplication_ecdsa_module a b result =
     let t = create (size 8) (u64 0) in 
     let round2 = create (size 8) (u64 0) in 
     let round4 = create (size 8) (u64 0) in  
-    let primeBuffer = create (size 4) (u64 0) in 
+    let prime_p256_orderBuffer = create (size 4) (u64 0) in 
 
-    upload_ecdsa_prime primeBuffer;
+    upload_ecdsa_prime_p256_order prime_p256_orderBuffer;
     let k0 = upload_k0() in 
     
       let h0 = ST.get() in     
     mul a b t;
       let h1 = ST.get() in 
-      mul_lemma_ (as_nat h0 a) (as_nat h0 b) prime;
-      assert(wide_as_nat h1 t < prime * prime);
+      mul_lemma_ (as_nat h0 a) (as_nat h0 b) prime_p256_order;
+      assert(wide_as_nat h1 t < prime_p256_order * prime_p256_order);
 
-   montgomery_multiplication_round_twice t round2 k0 primeBuffer; 
+   montgomery_multiplication_round_twice t round2 k0 prime_p256_orderBuffer; 
      let h2 = ST.get() in 
-   montgomery_multiplication_round_twice round2 round4 k0 primeBuffer;
+   montgomery_multiplication_round_twice round2 round4 k0 prime_p256_orderBuffer;
      let h3 = ST.get() in 
-     lemma_mod_mul_distr_l (wide_as_nat h2 round2) (modp_inv2_prime (pow2 128) prime) prime;
-     lemma_mod_mul_distr_l (as_nat h0 a * as_nat h0 b * modp_inv2_prime (pow2 128) prime) (modp_inv2_prime (pow2 128) prime) prime;
+     lemma_mod_mul_distr_l (wide_as_nat h2 round2) (modp_inv2_prime (pow2 128) prime_p256_order) prime_p256_order;
+     lemma_mod_mul_distr_l (as_nat h0 a * as_nat h0 b * modp_inv2_prime (pow2 128) prime_p256_order) (modp_inv2_prime (pow2 128) prime_p256_order) prime_p256_order;
      lemma_montgomery_mod_inverse_addition2 (as_nat h0 a * as_nat h0 b);
-     assert(wide_as_nat h3 round4 % prime == (as_nat h0 a * as_nat h0 b  * modp_inv2_prime (pow2 256) prime) % prime);
-     lemma_montgomery_mult_result_less_than_prime (as_nat h0 a) (as_nat h0 b) (uint_v k0);
-     assert(wide_as_nat h3 round4 < 2 * prime);
-     reduction_prime_2prime_with_carry_impl_5 round4 result primeBuffer; 
+     assert(wide_as_nat h3 round4 % prime_p256_order == (as_nat h0 a * as_nat h0 b  * modp_inv2_prime (pow2 256) prime_p256_order) % prime_p256_order);
+     lemma_montgomery_mult_result_less_than_prime_p256_order (as_nat h0 a) (as_nat h0 b) (uint_v k0);
+     assert(wide_as_nat h3 round4 < 2 * prime_p256_order);
+     reduction_prime_p256_order_2prime_p256_order_with_carry_impl_5 round4 result prime_p256_orderBuffer; 
       let h4 = ST.get() in 
-      assert(as_nat h4 result == wide_as_nat h3 round4 % prime);
-     assert(as_nat  h4 result == (as_nat h0 a * as_nat h0 b  * modp_inv2_prime (pow2 256) prime) % prime); 
+      assert(as_nat h4 result == wide_as_nat h3 round4 % prime_p256_order);
+     assert(as_nat  h4 result == (as_nat h0 a * as_nat h0 b  * modp_inv2_prime (pow2 256) prime_p256_order) % prime_p256_order); 
     pop_frame()
