code/experimental/P256/Hacl.Spec.P256.MontgomeryMultiplication.fsti
@@ -20,7 +20,7 @@ open Lib.Sequence
 
 
 noextract
-val fromDomain_: a: int -> Tot (r: nat (*{ r = a * modp_inv2 (pow2 256) % prime}*))
+val fromDomain_: a: int -> Tot (r: nat (*{ r = a * modp_inv2 (pow2 256) % prime256}*))
 
 noextract
 val fromDomainPoint: a: tuple3 nat nat nat -> Tot (r: tuple3 nat nat nat 
@@ -33,117 +33,117 @@ val fromDomainPoint: a: tuple3 nat nat nat -> Tot (r: tuple3 nat nat nat
 
 
 noextract
-val toDomain_: a: int -> Tot (r: nat (*{r =  a * pow2 256 % prime}*))
+val toDomain_: a: int -> Tot (r: nat (*{r =  a * pow2 256 % prime256}*))
 
-val lemmaFromDomain: a: int -> Lemma (fromDomain_ (a) == a * modp_inv2 (pow2 256) % prime)
+val lemmaFromDomain: a: int -> Lemma (fromDomain_ (a) == a * modp_inv2 (pow2 256) % prime256)
 
-val lemmaToDomain: a: int -> Lemma (toDomain_(a) == a * (pow2 256) % prime)
+val lemmaToDomain: a: int -> Lemma (toDomain_(a) == a * (pow2 256) % prime256)
 
-val lemmaToDomainAndBackIsTheSame: a: nat { a < prime} -> Lemma (fromDomain_ (toDomain_ a) == a)
+val lemmaToDomainAndBackIsTheSame: a: nat { a < prime256} -> Lemma (fromDomain_ (toDomain_ a) == a)
   [SMTPat (fromDomain_ (toDomain_ a))]
 
-val lemmaFromDomainToDomain: a: nat { a < prime} -> Lemma (toDomain_ (fromDomain_ a) == a)
+val lemmaFromDomainToDomain: a: nat { a < prime256} -> Lemma (toDomain_ (fromDomain_ a) == a)
 
-(* the lemma shows the equivalence between toDomain(a:nat) and toDomain(a % prime) *)
-val inDomain_mod_is_not_mod: a: int -> Lemma (toDomain_ a == toDomain_ (a % prime))
+(* the lemma shows the equivalence between toDomain(a:nat) and toDomain(a % prime256) *)
+val inDomain_mod_is_not_mod: a: int -> Lemma (toDomain_ a == toDomain_ (a % prime256))
 
-val additionInDomain2Nat: a: nat {a < prime} -> b: nat {b < prime} -> Lemma 
+val additionInDomain2Nat: a: nat {a < prime256} -> b: nat {b < prime256} -> Lemma 
   (
-    let result = (a + b) % prime in 
+    let result = (a + b) % prime256 in 
     result = toDomain_ (fromDomain_ a + fromDomain_ b)
   )
   
-val substractionInDomain2Nat: a: nat {a < prime} -> b: nat { b < prime} -> Lemma 
-  ((a - b) % prime == toDomain_ (fromDomain_ a - fromDomain_ b))
+val substractionInDomain2Nat: a: nat {a < prime256} -> b: nat { b < prime256} -> Lemma 
+  ((a - b) % prime256 == toDomain_ (fromDomain_ a - fromDomain_ b))
   
 
 noextract 
-val felem_add_seq: a: felem_seq{felem_seq_as_nat a < prime} -> b: felem_seq{felem_seq_as_nat b < prime} -> 
-  Tot (r: felem_seq {felem_seq_as_nat r < prime /\ 
-    felem_seq_as_nat r = toDomain_ ((fromDomain_ (felem_seq_as_nat a) + fromDomain_ (felem_seq_as_nat b)) % prime)})
+val felem_add_seq: a: felem_seq{felem_seq_as_nat a < prime256} -> b: felem_seq{felem_seq_as_nat b < prime256} -> 
+  Tot (r: felem_seq {felem_seq_as_nat r < prime256 /\ 
+    felem_seq_as_nat r = toDomain_ ((fromDomain_ (felem_seq_as_nat a) + fromDomain_ (felem_seq_as_nat b)) % prime256)})
 
 noextract
-val felem_sub_seq: a: felem_seq{felem_seq_as_nat a < prime} -> b: felem_seq{felem_seq_as_nat b < prime} -> 
-  Tot (r: felem_seq {felem_seq_as_nat r < prime /\ 
-  felem_seq_as_nat r = toDomain_ ((fromDomain_ (felem_seq_as_nat a) - fromDomain_(felem_seq_as_nat b))% prime)})
+val felem_sub_seq: a: felem_seq{felem_seq_as_nat a < prime256} -> b: felem_seq{felem_seq_as_nat b < prime256} -> 
+  Tot (r: felem_seq {felem_seq_as_nat r < prime256 /\ 
+  felem_seq_as_nat r = toDomain_ ((fromDomain_ (felem_seq_as_nat a) - fromDomain_(felem_seq_as_nat b))% prime256)})
 
 
 noextract
-val montgomery_multiplication_seq: a: felem_seq {felem_seq_as_nat a < prime} -> b: felem_seq {felem_seq_as_nat b < prime} -> Tot (r: felem_seq {felem_seq_as_nat r < prime /\ 
-  felem_seq_as_nat r = toDomain_ (fromDomain_ (felem_seq_as_nat a) * fromDomain_(felem_seq_as_nat b) % prime)
+val montgomery_multiplication_seq: a: felem_seq {felem_seq_as_nat a < prime256} -> b: felem_seq {felem_seq_as_nat b < prime256} -> Tot (r: felem_seq {felem_seq_as_nat r < prime256 /\ 
+  felem_seq_as_nat r = toDomain_ (fromDomain_ (felem_seq_as_nat a) * fromDomain_(felem_seq_as_nat b) % prime256)
   }) 
    
 val montgomery_multiplication_buffer: a: felem -> b: felem -> r: felem ->  Stack unit
-  (requires (fun h -> live h a /\ as_nat h a < prime /\ live h b /\ live h r /\ as_nat h b < prime)) 
+  (requires (fun h -> live h a /\ as_nat h a < prime256 /\ live h b /\ live h r /\ as_nat h b < prime256)) 
   (ensures (fun h0 _ h1 -> modifies1 r h0 h1 /\ 
-    as_nat h1 r < prime /\
+    as_nat h1 r < prime256 /\
     as_seq h1 r == montgomery_multiplication_seq (as_seq h0 a) (as_seq h0 b)))
 
 noextract
-val mm_cube_seq: a: felem_seq {felem_seq_as_nat a < prime}-> 
-  Tot (r: felem_seq {felem_seq_as_nat r < prime /\ 
-  felem_seq_as_nat r = toDomain_ (fromDomain_ (felem_seq_as_nat a) * fromDomain_ (felem_seq_as_nat a) * fromDomain_ (felem_seq_as_nat a) % prime) })
+val mm_cube_seq: a: felem_seq {felem_seq_as_nat a < prime256}-> 
+  Tot (r: felem_seq {felem_seq_as_nat r < prime256 /\ 
+  felem_seq_as_nat r = toDomain_ (fromDomain_ (felem_seq_as_nat a) * fromDomain_ (felem_seq_as_nat a) * fromDomain_ (felem_seq_as_nat a) % prime256) })
 
 noextract
-val mm_quatre_seq: a: felem_seq {felem_seq_as_nat a < prime} -> 
-  Tot (r: felem_seq {felem_seq_as_nat r < prime /\ 
-  felem_seq_as_nat r = toDomain_ (fromDomain_ (felem_seq_as_nat a) * fromDomain_ (felem_seq_as_nat a) * fromDomain_ (felem_seq_as_nat a) * fromDomain_ (felem_seq_as_nat a) % prime)})
+val mm_quatre_seq: a: felem_seq {felem_seq_as_nat a < prime256} -> 
+  Tot (r: felem_seq {felem_seq_as_nat r < prime256 /\ 
+  felem_seq_as_nat r = toDomain_ (fromDomain_ (felem_seq_as_nat a) * fromDomain_ (felem_seq_as_nat a) * fromDomain_ (felem_seq_as_nat a) * fromDomain_ (felem_seq_as_nat a) % prime256)})
 
 noextract 
-val mm_byTwo_seq: a: felem_seq {felem_seq_as_nat a < prime} -> Tot (r: felem_seq {felem_seq_as_nat r < prime /\
-  felem_seq_as_nat r = toDomain_ (2 * fromDomain_ (felem_seq_as_nat a) % prime)})
+val mm_byTwo_seq: a: felem_seq {felem_seq_as_nat a < prime256} -> Tot (r: felem_seq {felem_seq_as_nat r < prime256 /\
+  felem_seq_as_nat r = toDomain_ (2 * fromDomain_ (felem_seq_as_nat a) % prime256)})
 
 
-val lemma_add_same_value_is_by_two: a: felem_seq {felem_seq_as_nat a < prime} -> 
+val lemma_add_same_value_is_by_two: a: felem_seq {felem_seq_as_nat a < prime256} -> 
   Lemma (felem_add_seq a a  == mm_byTwo_seq a)
 
 noextract 
-val mm_byThree_seq: a: felem_seq {felem_seq_as_nat a < prime} -> Tot (r: felem_seq {felem_seq_as_nat r < prime /\
-  felem_seq_as_nat r = toDomain_ (3 * fromDomain_ (felem_seq_as_nat a) % prime )})
+val mm_byThree_seq: a: felem_seq {felem_seq_as_nat a < prime256} -> Tot (r: felem_seq {felem_seq_as_nat r < prime256 /\
+  felem_seq_as_nat r = toDomain_ (3 * fromDomain_ (felem_seq_as_nat a) % prime256 )})
 
 noextract 
-val mm_byFour_seq: a: felem_seq {felem_seq_as_nat a < prime} -> Tot (r: felem_seq {felem_seq_as_nat r < prime /\
-  felem_seq_as_nat r = toDomain_ (4 * fromDomain_ (felem_seq_as_nat a) % prime)})
+val mm_byFour_seq: a: felem_seq {felem_seq_as_nat a < prime256} -> Tot (r: felem_seq {felem_seq_as_nat r < prime256 /\
+  felem_seq_as_nat r = toDomain_ (4 * fromDomain_ (felem_seq_as_nat a) % prime256)})
 
 noextract 
-val mm_byEight_seq: a: felem_seq {felem_seq_as_nat a < prime} -> Tot (r: felem_seq {felem_seq_as_nat r < prime /\
-  felem_seq_as_nat r = toDomain_ (8 * fromDomain_ (felem_seq_as_nat a) % prime)})
+val mm_byEight_seq: a: felem_seq {felem_seq_as_nat a < prime256} -> Tot (r: felem_seq {felem_seq_as_nat r < prime256 /\
+  felem_seq_as_nat r = toDomain_ (8 * fromDomain_ (felem_seq_as_nat a) % prime256)})
 
 
-val lemma_add_same_value_is_by_three: a: felem_seq {felem_seq_as_nat a < prime} -> 
+val lemma_add_same_value_is_by_three: a: felem_seq {felem_seq_as_nat a < prime256} -> 
   Lemma (let two = mm_byTwo_seq a in let three = felem_add_seq a two in three  == mm_byThree_seq a)
 
 
-val lemma_add_same_value_is_by_four: a: felem_seq {felem_seq_as_nat a < prime} -> 
+val lemma_add_same_value_is_by_four: a: felem_seq {felem_seq_as_nat a < prime256} -> 
   Lemma (let two = mm_byTwo_seq a in let four = mm_byTwo_seq two  in four  == mm_byFour_seq a)
 
 
-val lemma_add_same_value_is_by_eight: a: felem_seq {felem_seq_as_nat a < prime} -> 
+val lemma_add_same_value_is_by_eight: a: felem_seq {felem_seq_as_nat a < prime256} -> 
   Lemma (let two = mm_byTwo_seq a in let four = mm_byTwo_seq two in let eight = mm_byTwo_seq four in eight  == mm_byEight_seq a)
 
 
 noextract 
-val mm_byMinusThree_seq: a: felem_seq {felem_seq_as_nat a < prime} -> Tot (r: felem_seq {felem_seq_as_nat r < prime /\
-  felem_seq_as_nat r = toDomain_ ((-3) * fromDomain_ (felem_seq_as_nat a) % prime)})
+val mm_byMinusThree_seq: a: felem_seq {felem_seq_as_nat a < prime256} -> Tot (r: felem_seq {felem_seq_as_nat r < prime256 /\
+  felem_seq_as_nat r = toDomain_ ((-3) * fromDomain_ (felem_seq_as_nat a) % prime256)})
 
 
-val lemma_add_same_value_is_by_minus_three: a: felem_seq{felem_seq_as_nat a < prime} -> zero: felem_seq{felem_seq_as_nat zero = 0} ->
+val lemma_add_same_value_is_by_minus_three: a: felem_seq{felem_seq_as_nat a < prime256} -> zero: felem_seq{felem_seq_as_nat zero = 0} ->
   Lemma ( 
       let three = mm_byThree_seq a in 
       let minusThree = felem_sub_seq zero three in 
       minusThree == mm_byMinusThree_seq a)
 
 
-val lemmaEraseToDomainFromDomain: z: nat-> Lemma (toDomain_ (fromDomain_ (toDomain_ (z * z % prime)) * z % prime) == toDomain_ (z * z * z % prime))
+val lemmaEraseToDomainFromDomain: z: nat-> Lemma (toDomain_ (fromDomain_ (toDomain_ (z * z % prime256)) * z % prime256) == toDomain_ (z * z * z % prime256))
 
 val exponent: a: felem ->result: felem -> tempBuffer: lbuffer uint64 (size 20) ->  Stack unit
   (requires fun h -> live h a /\ live h tempBuffer /\ live h result /\ disjoint tempBuffer result /\ 
-  disjoint a tempBuffer /\ as_nat h a < prime)
+  disjoint a tempBuffer /\ as_nat h a < prime256)
   (ensures fun h0 _ h1 -> modifies2 result tempBuffer h0 h1 /\ (let k = fromDomain_ (as_nat h0 a) in 
-    as_nat h1 result =  toDomain_ ((pow k (prime-2)) % prime)))
+    as_nat h1 result =  toDomain_ ((pow k (prime256-2)) % prime256)))
 
 
 val clean_exponent: a: felem -> result: felem -> tempBuffer: lbuffer uint64 (size 20) -> Stack unit
   (requires fun h -> live h a  /\ live h result /\ live h tempBuffer /\ disjoint tempBuffer result /\
-    disjoint a tempBuffer /\ as_nat h a < prime)
+    disjoint a tempBuffer /\ as_nat h a < prime256)
   (ensures fun h0 _ h1 -> True) 
