code/experimental/P256/Hacl.Spec.ECDSA.fst
@@ -1,0 +1,20 @@
+module Hacl.Spec.ECDSA
+
+open FStar.Mul 
+open Hacl.Spec.P256.Definitions
+open Hacl.Spec.P256.Lemmas
+
+open Lib.ByteSequence
+open Lib.IntTypes
+open Lib.Sequence
+
+
+
+
+let scalar = lbytes 32
+
+let ith_bit (k:lbytes 32) (i:nat{i < 256}) : uint64 =
+  let q = i / 8 in let r = size (i % 8) in
+  to_u64 ((index k q >>. r) &. u8 1)
+
+
