code/experimental/P256/Hacl.Spec.P256.Core.fsti
@@ -16,19 +16,19 @@ inline_for_extraction noextract
 val eq_0_u64: a: uint64 -> Tot (r: bool {if uint_v a = 0 then r == true else r == false})
 
 inline_for_extraction noextract
-val felem_add: arg1: felem4 {as_nat4 arg1 < prime} -> arg2: felem4{as_nat4 arg2 < prime} -> Tot (r : felem4 {as_nat4 r == (as_nat4 arg1 + as_nat4 arg2) % prime})
+val felem_add: arg1: felem4 {as_nat4 arg1 < prime256} -> arg2: felem4{as_nat4 arg2 < prime256} -> Tot (r : felem4 {as_nat4 r == (as_nat4 arg1 + as_nat4 arg2) % prime256})
 
 inline_for_extraction noextract
-val felem_sub: arg1: felem4 {as_nat4 arg1 < prime} -> arg2: felem4 {as_nat4 arg2 < prime} -> Tot (r : felem4 {as_nat4 r < prime /\ as_nat4 r == (as_nat4 arg1 - as_nat4 arg2) % prime})
+val felem_sub: arg1: felem4 {as_nat4 arg1 < prime256} -> arg2: felem4 {as_nat4 arg2 < prime256} -> Tot (r : felem4 {as_nat4 r < prime256 /\ as_nat4 r == (as_nat4 arg1 - as_nat4 arg2) % prime256})
 
 inline_for_extraction noextract
-val reduction_prime_2prime: a: felem4 -> Tot (r:felem4{as_nat4 r == as_nat4 a % prime})
+val reduction_prime_2prime: a: felem4 -> Tot (r:felem4{as_nat4 r == as_nat4 a % prime256})
 
 inline_for_extraction noextract 
-val shift_left_felem: input: felem4{as_nat4 input < prime} -> Tot (r: felem4 {as_nat4 r == (as_nat4 input * 2) % prime})
+val shift_left_felem: input: felem4{as_nat4 input < prime256} -> Tot (r: felem4 {as_nat4 r == (as_nat4 input * 2) % prime256})
 
 inline_for_extraction noextract
-val upload_prime: unit -> Tot (r: felem4 {as_nat4 r = prime})
+val upload_prime: unit -> Tot (r: felem4 {as_nat4 r = prime256})
 
 inline_for_extraction noextract 
 val shift_256: c: felem4 -> Tot (r: felem8{wide_as_nat4 r = as_nat4 c * pow2 256})
@@ -44,26 +44,26 @@ inline_for_extraction noextract
 val add8_without_carry1: a: felem8{wide_as_nat4 a < pow2 449} -> b: felem8 {wide_as_nat4 b < pow2 320} -> Tot (r: felem8 {wide_as_nat4 r = wide_as_nat4 a + wide_as_nat4 b})
 
 inline_for_extraction noextract
-val montgomery_multiplication: a: felem4 {as_nat4 a < prime} -> b: felem4{as_nat4 b < prime}  -> 
-  Tot (result: felem4 {as_nat4 result = as_nat4 a * as_nat4 b * modp_inv2 (pow2 256) % prime})
+val montgomery_multiplication: a: felem4 {as_nat4 a < prime256} -> b: felem4{as_nat4 b < prime256}  -> 
+  Tot (result: felem4 {as_nat4 result = as_nat4 a * as_nat4 b * modp_inv2 (pow2 256) % prime256})
 
 inline_for_extraction noextract
-val cube_tuple: a: felem4{as_nat4 a < prime} -> Tot (result: felem4{as_nat4 result = (as_nat4 a * as_nat4 a * as_nat4 a * modp_inv2(pow2 256) * modp_inv2 (pow2 256)) % prime})
+val cube_tuple: a: felem4{as_nat4 a < prime256} -> Tot (result: felem4{as_nat4 result = (as_nat4 a * as_nat4 a * as_nat4 a * modp_inv2(pow2 256) * modp_inv2 (pow2 256)) % prime256})
 
 inline_for_extraction noextract
-val quatre_tuple: a: felem4 {as_nat4 a < prime} -> Tot (result : felem4 {as_nat4 result = (as_nat4 a * as_nat4 a * as_nat4 a * as_nat4 a * modp_inv2 (pow2 256) * modp_inv2 (pow2 256) * modp_inv2(pow2 256)) % prime})
+val quatre_tuple: a: felem4 {as_nat4 a < prime256} -> Tot (result : felem4 {as_nat4 result = (as_nat4 a * as_nat4 a * as_nat4 a * as_nat4 a * modp_inv2 (pow2 256) * modp_inv2 (pow2 256) * modp_inv2(pow2 256)) % prime256})
 
 inline_for_extraction noextract
-val multByThree_tuple: a: felem4{as_nat4 a < prime}  -> Tot (result: felem4{as_nat4 result = (as_nat4 a * 3) % prime})
+val multByThree_tuple: a: felem4{as_nat4 a < prime256}  -> Tot (result: felem4{as_nat4 result = (as_nat4 a * 3) % prime256})
 
 inline_for_extraction noextract
-val multByFour_tuple: a: felem4{as_nat4 a < prime} -> Tot (result : felem4 {as_nat4 result = (as_nat4 a * 4) % prime})
+val multByFour_tuple: a: felem4{as_nat4 a < prime256} -> Tot (result : felem4 {as_nat4 result = (as_nat4 a * 4) % prime256})
 
 inline_for_extraction noextract
-val multByEight_tuple: a: felem4 {as_nat4 a < prime} -> Tot (result: felem4 {as_nat4 result = (as_nat4 a * 8) % prime})
+val multByEight_tuple: a: felem4 {as_nat4 a < prime256} -> Tot (result: felem4 {as_nat4 result = (as_nat4 a * 8) % prime256})
 
 inline_for_extraction noextract
-val multByMinusThree_tuple: a: felem4 {as_nat4 a < prime} -> Tot (result: felem4 {as_nat4 result = (as_nat4 a * (-3)) % prime})
+val multByMinusThree_tuple: a: felem4 {as_nat4 a < prime256} -> Tot (result: felem4 {as_nat4 result = (as_nat4 a * (-3)) % prime256})
 
 inline_for_extraction noextract
 val isOne_tuple: a: felem4 -> Tot (r: bool {if as_nat4 a = 1 then r == true else r == false})
